examples/bw/BW1.v
@@ -46,9 +46,11 @@ Section BW.
     ]
   .
 
-  Definition BWSem: ModSemL.t := {|
-    ModSemL.fnsems := List.map (fun '(fn, fsb) => (fn, fun_to_tgt BWStb fn fsb)) BWSbtb;
-    ModSemL.initial_mrs := [("BW", (GRA.embed (bw_full false), tt↑))];
+  Definition BWSem: ModSem.t := {|
+    ModSem.fnsems := List.map (fun '(fn, fsb) => (fn, fun_to_tgt BWStb fn fsb)) BWSbtb;
+    ModSem.mn := "BW";
+    ModSem.initial_mr := GRA.embed (bw_full false);
+    ModSem.initial_st := tt↑;
   |}
   .
 
